src/Common/OneDiskAPI.v
@@ -8,7 +8,7 @@ Definition read_spec (a : addr) : Specification _ block unit State :=
     pre := True;
     post := fun r state' =>
       state' = state /\
-      state a ?|= eq r;
+      diskGet state a ?|= eq r;
     recover := fun _ state' =>
       state' = state
   |}.
@@ -22,11 +22,11 @@ Definition write_spec (a : addr) (v : block) : Specification _ _ unit State :=
       state' = state \/ state' = diskUpd state a v
   |}.
 
-Definition diskSize_spec : Specification _ nat unit State :=
+Definition size_spec : Specification _ nat unit State :=
   fun (_ : unit) state => {|
     pre := True;
     post := fun r state' =>
-      state' = state /\ r = size state;
+      state' = state /\ r = diskSize state;
     recover := fun _ state' =>
       state' = state
   |}.
@@ -37,7 +37,7 @@ Module Type OneDiskAPI.
   Parameter init : prog InitResult.
   Parameter read : addr -> prog block.
   Parameter write : addr -> block -> prog unit.
-  Parameter diskSize : prog nat.
+  Parameter size : prog nat.
   Parameter recover : prog unit.
 
   Axiom abstr : Abstraction State.
@@ -45,13 +45,13 @@ Module Type OneDiskAPI.
   Axiom init_ok : init_abstraction init recover abstr inited_any.
   Axiom read_ok : forall a, prog_spec (read_spec a) (read a) recover abstr.
   Axiom write_ok : forall a v, prog_spec (write_spec a v) (write a v) recover abstr.
-  Axiom diskSize_ok : prog_spec diskSize_spec diskSize recover abstr.
+  Axiom size_ok : prog_spec size_spec size recover abstr.
   Axiom recover_noop : rec_noop recover abstr no_wipe.
 
   Hint Resolve init_ok.
   Hint Resolve read_ok.
   Hint Resolve write_ok.
-  Hint Resolve diskSize_ok.
+  Hint Resolve size_ok.
   Hint Resolve recover_noop.
 
 End OneDiskAPI.
