src/Lab4/TwoDiskAPI.v
@@ -18,7 +18,7 @@ Definition read_spec (i : diskId) (a : addr) : Specification _ _ unit _ :=
       | Working v =>
         get_disk i         state' ?|= eq d /\
         get_disk (other i) state' ?|= F /\
-        d a ?|= eq v
+        diskGet d a ?|= eq v
       | Failed =>
         get_disk i         state' ?|= missing /\
         get_disk (other i) state' ?|= F
@@ -44,11 +44,11 @@ Definition write_spec (i : diskId) (a : addr) (b : block) : Specification _ (Dis
       end;
     recover := fun _ state' =>
       (get_disk i state' ?|= eq d \/
-       get_disk i state' ?|= eq (diskUpd d a b) /\ a < size d) /\
+       get_disk i state' ?|= eq (diskUpd d a b) /\ a < diskSize d) /\
       get_disk (other i) state' ?|= F;
   |}.
 
-Definition diskSize_spec (i : diskId) : Specification _ _ unit _ :=
+Definition size_spec (i : diskId) : Specification _ _ unit _ :=
   fun '(d, F) state => {|
     pre :=
       get_disk i         state ?|= eq d /\
@@ -58,7 +58,7 @@ Definition diskSize_spec (i : diskId) : Specification _ _ unit _ :=
       | Working n =>
         get_disk i         state' ?|= eq d /\
         get_disk (other i) state' ?|= F /\
-        n = size d
+        n = diskSize d
       | Failed =>
         get_disk i         state' ?|= missing /\
         get_disk (other i) state' ?|= F
@@ -74,7 +74,7 @@ Module Type TwoDiskAPI.
   Parameter init : prog InitResult.
   Parameter read : diskId -> addr -> prog (DiskResult block).
   Parameter write : diskId -> addr -> block -> prog (DiskResult unit).
-  Parameter diskSize : diskId -> prog (DiskResult nat).
+  Parameter size : diskId -> prog (DiskResult nat).
   Parameter recover : prog unit.
 
   Axiom abstr : Abstraction State.
@@ -82,13 +82,13 @@ Module Type TwoDiskAPI.
   Axiom init_ok : init_abstraction init recover abstr inited_any.
   Axiom read_ok : forall i a, prog_spec (read_spec i a) (read i a) recover abstr.
   Axiom write_ok : forall i a v, prog_spec (write_spec i a v) (write i a v) recover abstr.
-  Axiom diskSize_ok : forall i, prog_spec (diskSize_spec i) (diskSize i) recover abstr.
+  Axiom size_ok : forall i, prog_spec (size_spec i) (size i) recover abstr.
   Axiom recover_noop : rec_noop recover abstr no_wipe.
 
   Hint Resolve init_ok.
   Hint Resolve read_ok.
   Hint Resolve write_ok.
-  Hint Resolve diskSize_ok.
+  Hint Resolve size_ok.
   Hint Resolve recover_noop.
 
 End TwoDiskAPI.
