src/Lab2/BadSectorImpl.v
@@ -10,7 +10,7 @@ Module BadSectorDisk <: BadSectorAPI.
   Axiom read : addr -> prog block.
   Axiom write : addr -> block -> prog unit.
   Axiom getBadSector : prog addr.
-  Axiom diskSize : prog nat.
+  Axiom size : prog nat.
   Axiom recover : prog unit.
 
   Axiom abstr : Abstraction State.
@@ -19,7 +19,7 @@ Module BadSectorDisk <: BadSectorAPI.
   Axiom read_ok : forall a, prog_spec (read_spec a) (read a) recover abstr.
   Axiom write_ok : forall a v, prog_spec (write_spec a v) (write a v) recover abstr.
   Axiom getBadSector_ok : prog_spec getBadSector_spec getBadSector recover abstr.
-  Axiom diskSize_ok : prog_spec diskSize_spec diskSize recover abstr.
+  Axiom size_ok : prog_spec size_spec size recover abstr.
   Axiom recover_noop : rec_noop recover abstr no_wipe.
 
 End BadSectorDisk.
@@ -27,4 +27,4 @@ End BadSectorDisk.
 Extract Constant BadSectorDisk.read => "BadSectorDisk.Ops.read".
 Extract Constant BadSectorDisk.write => "BadSectorDisk.Ops.write".
 Extract Constant BadSectorDisk.getBadSector => "BadSectorDisk.Ops.getBadSector".
-Extract Constant BadSectorDisk.diskSize => "BadSectorDisk.Ops.diskSize".
+Extract Constant BadSectorDisk.size => "BadSectorDisk.Ops.size".
