src/Lab4/TwoDiskBaseImpl.v
@@ -9,7 +9,7 @@ Module TwoDiskBase <: TwoDiskBaseAPI.
   Axiom init : prog InitResult.
   Axiom read : diskId -> addr -> prog (DiskResult block).
   Axiom write : diskId -> addr -> block -> prog (DiskResult unit).
-  Axiom diskSize : diskId -> prog (DiskResult nat).
+  Axiom size : diskId -> prog (DiskResult nat).
   Axiom recover : prog unit.
 
   Axiom abstr : Abstraction State.
@@ -17,11 +17,11 @@ Module TwoDiskBase <: TwoDiskBaseAPI.
   Axiom init_ok : init_abstraction init recover abstr inited_any.
   Axiom read_ok : forall i a, prog_spec (op_spec (combined_step (op_read i a))) (read i a) recover abstr.
   Axiom write_ok : forall i a b, prog_spec (op_spec (combined_step (op_write i a b))) (write i a b) recover abstr.
-  Axiom diskSize_ok : forall i, prog_spec (op_spec (combined_step (op_disksize i))) (diskSize i) recover abstr.
+  Axiom size_ok : forall i, prog_spec (op_spec (combined_step (op_size i))) (size i) recover abstr.
   Axiom recover_noop : rec_noop recover abstr no_wipe.
 
 End TwoDiskBase.
 
 Extract Constant TwoDiskBase.read => "TD.read".
 Extract Constant TwoDiskBase.write => "TD.write".
-Extract Constant TwoDiskBase.diskSize => "TD.diskSize".
+Extract Constant TwoDiskBase.size => "TD.size".
